Solution.v
@@ -1,1 +1,100 @@
-Require Import Preloaded.
+Require Import Preloaded VST.floyd.proofauto VST.floyd.library.
+
+Lemma listrep_local_prop: forall il p, listrep il p |--
+        !! (is_pointer_or_null p  /\ (p=nullval <-> il=nil)).
+Proof.
+  induction il; intros; unfold listrep; fold listrep.
+  - entailer!; split; auto.
+  - Intros y.
+    entailer!.
+    split; intros; try discriminate; subst p.
+    eapply field_compatible_nullval; eauto.
+Qed.
+#[export] Hint Resolve listrep_local_prop : saturate_local.
+
+Lemma listrep_valid_pointer:
+  forall il p,
+   listrep il p |-- valid_pointer p.
+Proof.
+  destruct il; intros; unfold listrep; fold listrep.
+  - entailer!.
+  - Intros y; entailer!.
+Qed.
+#[export] Hint Resolve listrep_valid_pointer : valid_pointer.
+
+Lemma queue_local_prop: forall il p, queue il p |--  !! (isptr p).
+Proof.
+  intros; unfold queue.
+  destruct il.
+  - entailer!.
+  - Intros front back; entailer!.
+Qed.
+#[export] Hint Resolve queue_local_prop : saturate_local.
+
+Lemma queue_valid_pointer:
+  forall il p,
+   queue il p |-- valid_pointer p.
+Proof.
+  intros; unfold queue.
+  destruct il.
+  - entailer!.
+  - Intros front back; entailer!.
+Qed.
+#[export] Hint Resolve queue_valid_pointer : valid_pointer.
+
+Lemma body_queue_init : semax_body Vprog Gprog f_queue_init queue_init_spec.
+Proof. start_function; do 3 forward; unfold queue; entailer!. Qed.
+
+Lemma body_queue_is_empty :
+  semax_body Vprog Gprog f_queue_is_empty queue_is_empty_spec.
+Proof.
+  start_function.
+  unfold queue.
+  destruct il.
+  - do 2 forward.
+  - Intros front back.
+    forward.
+    + unfold listrep; fold listrep.
+      Intros y y0; subst y0.
+      autorewrite with norm.
+      assert_PROP (isptr front) by (rewrite (data_at_isptr _ _ _ front);
+        entailer!).
+      entailer!.
+    + forward.
+      unfold queue; unfold listrep; fold listrep.
+      Intros y y0; subst y0.
+      destruct (eq_dec (z :: il) []) as [Econtra | E]; try discriminate; clear E.
+      Exists front back y nullval.
+      assert_PROP (isptr front) by (rewrite (data_at_isptr _ _ _ front);
+        entailer!).
+      entailer!.
+      destruct front; unfold isptr in H1; try now exfalso.
+      auto.
+Qed.
+
+Lemma body_queue_front : semax_body Vprog Gprog f_queue_front queue_front_spec.
+Proof.
+  start_function.
+  unfold queue; unfold listrep; fold listrep.
+  Intros front back y y0; subst y0.
+  forward.
+  - autorewrite with norm.
+    assert_PROP (isptr front) by (rewrite (data_at_isptr _ _ _ front);
+      entailer!).
+    entailer!.
+  - autorewrite with norm.
+    Fail forward.
+    admit.
+Admitted.
+
+Lemma body_queue_enqueue :
+  semax_body Vprog Gprog f_queue_enqueue queue_enqueue_spec.
+Proof.
+  start_function.
+Admitted.
+
+Lemma body_queue_dequeue :
+  semax_body Vprog Gprog f_queue_dequeue queue_dequeue_spec.
+Proof.
+  start_function.
+Admitted.
